DeBruijnSSA/BinSyntax/Rewrite/Term/Compose/Structural/Product.lean
@@ -10,8 +10,8 @@ namespace Term
 def Eqv.pack {Γ : Ctx α ε} (h : ∀i, Γ.effect i ≤ e) : Eqv φ Γ (Γ.pack, e) := match Γ with
   | [] => unit e
   | V::Γ => pair
-    (var 0 (Ctx.Var.head (by constructor; rfl; convert (h 0); simp) _))
     ((pack (Γ := Γ) (λi => by convert h (i + 1) using 1; simp)).wk0)
+    (var 0 (Ctx.Var.head (by constructor; rfl; convert (h 0); simp) _))
 
 theorem Eqv.pack_def {Γ : Ctx α ε} {h : ∀i, Γ.effect i ≤ e}
   : Eqv.pack (φ := φ) (Γ := Γ) h = ⟦Term.InS.pack h⟧ := by
@@ -26,7 +26,7 @@ theorem Eqv.packE_def' {Γ : Ctx α ε} {h : Γ.Pure} : h.packE (φ := φ) = ⟦
   simp only [Ctx.Pure.packE, pack_def]
 
 theorem Eqv.packE_cons {Γ : Ctx α ε} {h : Ctx.Pure (V::Γ)}
-  : h.packE (φ := φ) = pair (var 0 (h.any_effect_refl (by simp))) h.tail.packE.wk0
+  : h.packE (φ := φ) = pair h.tail.packE.wk0 (var 0 (h.any_effect_refl (by simp)))
   := rfl
 
 @[simp]
@@ -51,7 +51,7 @@ theorem Eqv.Pure.pack_drop {Γ Δ : Ctx α ε} {i : Fin Γ.length}
   := ⟨Eqv.pack_drop i, rfl⟩
 
 def Eqv.pack_drop' {Γ Δ : Ctx α ε} (i : Fin Γ.length)
-  : Eqv φ ((Γ.pack, ⊥)::Δ) ((Γ.get i).1.prod (Ctx.pack (Γ.drop (i + 1))), e)
+  : Eqv φ ((Γ.pack, ⊥)::Δ) ((Ctx.pack (Γ.drop (i + 1))).prod (Γ.get i).1, e)
   := ⟦InS.pack_drop' i⟧
 
 theorem Eqv.Pure.pack_drop' {Γ Δ : Ctx α ε} {i : Fin Γ.length}
@@ -69,7 +69,7 @@ theorem Eqv.cast_pack_drop' {Γ Δ : Ctx α ε} {i : Fin Γ.length}
 
 def Eqv.pack_drop_succ {Γ Δ : Ctx α ε} (i : Fin Γ.length)
   : pack_drop (φ := φ)  (Γ := V::Γ) (Δ := Δ) (e := e) i.succ
-  = (pack_drop' (φ := φ) (Γ := V::Γ) (Δ := Δ) (e := e) i.castSucc).pr := by
+  = (pack_drop' (φ := φ) (Γ := V::Γ) (Δ := Δ) (e := e) i.castSucc).pl := by
   simp only [pack_drop, InS.pack_drop_succ]; rfl
 
 def Eqv.pi_n {Γ Δ : Ctx α ε} (i : Fin Γ.length) : Eqv φ ((Γ.pack, ⊥)::Δ) ((Γ.get i).1, e)
@@ -106,51 +106,51 @@ theorem Eqv.subst_lift_pi_n {Γ Δ Δ' : Ctx α ε} {i : Fin Γ.length} {σ : Su
   simp [pi_n]
 
 @[simp]
-theorem Eqv.subst0_nil_pr_pi_n {Γ Δ : Ctx α ε} {i : Fin Γ.length}
-  : (Eqv.pi_n (φ := φ) (Γ := Γ) (e := e) i).subst (nil.pr.subst0)
+theorem Eqv.subst0_nil_pl_pi_n {Γ Δ : Ctx α ε} {i : Fin Γ.length}
+  : (Eqv.pi_n (φ := φ) (Γ := Γ) (e := e) i).subst (nil.pl.subst0)
   = pi_n (φ := φ) (Γ := V::Γ) (Δ := Δ) i.succ := by
   apply eq_of_term_eq
-  apply Term.subst0_nil_pr_pi_n
+  apply Term.subst0_nil_pl_pi_n
 
 @[simp]
-theorem Eqv.subst0_pi_r_pi_n {Γ Δ : Ctx α ε} {i : Fin Γ.length}
-  : (Eqv.pi_n (φ := φ) (Γ := Γ) (e := e) i).subst pi_r.subst0
-  = pi_n (φ := φ) (Γ := V::Γ) (Δ := Δ) i.succ := subst0_nil_pr_pi_n
+theorem Eqv.subst0_pi_l_pi_n {Γ Δ : Ctx α ε} {i : Fin Γ.length}
+  : (Eqv.pi_n (φ := φ) (Γ := Γ) (e := e) i).subst pi_l.subst0
+  = pi_n (φ := φ) (Γ := V::Γ) (Δ := Δ) i.succ := subst0_nil_pl_pi_n
 
-theorem Eqv.pl_pack_drop'  {Γ Δ : Ctx α ε} {i : Fin Γ.length}
-  : (Eqv.pack_drop' (φ := φ) (Δ := Δ) (e := e) i).pl = pi_n i := rfl
+theorem Eqv.pr_pack_drop'  {Γ Δ : Ctx α ε} {i : Fin Γ.length}
+  : (Eqv.pack_drop' (φ := φ) (Δ := Δ) (e := e) i).pr = pi_n i := rfl
 
 theorem Eqv.pi_n_def {Γ Δ : Ctx α ε} (i : Fin Γ.length) :
   Eqv.pi_n (φ := φ) (Δ := Δ) (e := e) i = ⟦Term.InS.pi_n i⟧ := rfl
 
 theorem Eqv.pi_n_zero {Γ Δ : Ctx α ε}
-  : Eqv.pi_n (φ := φ) (Γ := V::Γ) (Δ := Δ) (e := e) (0 : Fin (Γ.length + 1)) = pi_l := rfl
+  : Eqv.pi_n (φ := φ) (Γ := V::Γ) (Δ := Δ) (e := e) (0 : Fin (Γ.length + 1)) = pi_r := rfl
 
 theorem Eqv.pi_n_succ {Γ Δ : Ctx α ε} (i : Fin Γ.length)
-  : pi_n (φ := φ) (Γ := V::Γ) (Δ := Δ) (e := e) i.succ = pi_r ;;' pi_n i := by
-  rw [seq, <-wk_eff_pi_r, let1_beta, wk1_pi_n, subst0_pi_r_pi_n]
+  : pi_n (φ := φ) (Γ := V::Γ) (Δ := Δ) (e := e) i.succ = pi_l ;;' pi_n i := by
+  rw [seq, <-wk_eff_pi_l, let1_beta, wk1_pi_n, subst0_pi_l_pi_n]
 
 theorem Eqv.pi_n_one {Γ Δ : Ctx α ε}
   : Eqv.pi_n (φ := φ) (Γ := V::V'::Γ) (Δ := Δ) (e := e) (1 : Fin (Γ.length + 2))
-  = pi_r ;;' pi_l := by exact pi_n_succ (Γ := V'::Γ) (0 : Fin (Γ.length + 1))
+  = pi_l ;;' pi_r := by exact pi_n_succ (Γ := V'::Γ) (0 : Fin (Γ.length + 1))
 
-def Eqv.pi_n' {Γ Δ : Ctx α ε} (i : Fin Γ.length) : Eqv φ ((Γ.pack, ⊥)::Δ) ((Γ.get i).1, e)
-  := match Γ with
-  | [] => i.elim0
-  | V::Γ => let2
-    (var (V := (V.1.prod (Ctx.pack Γ), e)) 0 (by simp [Ctx.pack]))
-    (i.cases (var 1 (by simp)) (λi => pi_n' i))
+-- def Eqv.pi_n' {Γ Δ : Ctx α ε} (i : Fin Γ.length) : Eqv φ ((Γ.pack, ⊥)::Δ) ((Γ.get i).1, e)
+--   := match Γ with
+--   | [] => i.elim0
+--   | V::Γ => let2
+--     (var (V := (V.1.prod (Ctx.pack Γ), e)) 0 (by simp [Ctx.pack]))
+--     (i.cases (var 1 (by simp)) (λi => pi_n' i))
 
-theorem Eqv.pi_n_def' {Γ Δ : Ctx α ε} (i : Fin Γ.length) :
-  pi_n' (φ := φ) (Δ := Δ) (e := e) i = ⟦Term.InS.pi_n' i⟧ := by
-  induction Γ generalizing Δ with
-  | nil => exact i.elim0
-  | cons _ _ I =>
-    simp only [
-      List.get_eq_getElem, List.length_cons, pi_n', var, Fin.val_zero,
-      List.getElem_cons_zero, I, InS.pi_n'
-    ]
-    cases i using Fin.cases <;> rfl
+-- theorem Eqv.pi_n_def' {Γ Δ : Ctx α ε} (i : Fin Γ.length) :
+--   pi_n' (φ := φ) (Δ := Δ) (e := e) i = ⟦Term.InS.pi_n' i⟧ := by
+--   induction Γ generalizing Δ with
+--   | nil => exact i.elim0
+--   | cons _ _ I =>
+--     simp only [
+--       List.get_eq_getElem, List.length_cons, pi_n', var, Fin.val_zero,
+--       List.getElem_cons_zero, I, InS.pi_n'
+--     ]
+--     cases i using Fin.cases <;> rfl
 
 def Subst.Eqv.unpack {Γ Δ : Ctx α ε} : Subst.Eqv φ ((Γ.pack, ⊥)::Δ) Γ := ⟦Subst.InS.unpack⟧
 
@@ -176,6 +176,52 @@ def Eqv.packed {Γ Δ : Ctx α ε} (a : Eqv φ Γ V) : Eqv φ ((Γ.pack, ⊥)::�
 theorem Eqv.packed_pair {Γ Δ : Ctx α ε} {A B : Ty α} {a : Eqv φ Γ (A, e)} {b : Eqv φ Γ (B, e)}
   : (pair a b).packed (Δ := Δ) = pair a.packed b.packed := by simp [packed]
 
+@[simp]
+theorem Eqv.wk_lift_packed {Γ Δ : Ctx α ε} {A : Ty α} {a : Eqv φ Γ (A, e)} {ρ : Ctx.InS Δ' Δ}
+  : (a.packed).wk (ρ.lift (le_refl _)) = a.packed := by
+  induction a using Quotient.inductionOn
+  apply eq_of_term_eq
+  simp only [Set.mem_setOf_eq, InS.coe_wk, Ctx.InS.coe_wk1, InS.coe_subst, Subst.InS.coe_unpack, ←
+    Term.subst_fromWk, Term.subst_subst, Ctx.InS.coe_lift]
+  congr
+  funext k; simp only [Subst.comp, Term.subst_fromWk, Term.wk_lift_pi_n, Subst.pi_n]
+
+@[simp]
+theorem Eqv.wk_liftn₂_packed {Γ Δ : Ctx α ε} {A : Ty α} {a : Eqv φ Γ (A, e)} {ρ : Ctx.InS Δ' Δ}
+  : (a.packed (Δ := V::Δ)).wk (ρ.liftn₂ (le_refl _) (le_refl _)) = a.packed := by
+  simp [<-Ctx.InS.lift_lift]
+
+@[simp]
+theorem Eqv.subst_lift_packed {Γ Δ Δ' : Ctx α ε} {A : Ty α} {a : Eqv φ Γ (A, e)}
+  {σ : Subst.Eqv φ Δ' Δ} : (a.packed).subst (σ.lift (le_refl _)) = a.packed := by
+  induction a using Quotient.inductionOn
+  induction σ using Quotient.inductionOn
+  apply eq_of_term_eq
+  simp only [Set.mem_setOf_eq, InS.coe_subst, Subst.InS.coe_lift, InS.coe_wk, Subst.InS.coe_unpack,
+    ←Term.subst_fromWk, Term.subst_subst]
+  congr
+  funext k; simp only [Subst.comp, Term.subst_fromWk, Term.subst_lift_pi_n, Subst.pi_n]
+
+@[simp]
+theorem Eqv.subst_liftn₂_packed {Γ Δ Δ' : Ctx α ε} {A : Ty α} {a : Eqv φ Γ (A, e)}
+  {σ : Subst.Eqv φ Δ' Δ}
+  : (a.packed (Δ := V::Δ)).subst (σ.liftn₂ (le_refl _) (le_refl _)) = a.packed := by
+  simp [<-Subst.Eqv.lift_lift]
+
+@[simp]
+theorem Eqv.wk1_packed {Γ Δ : Ctx α ε} {A : Ty α} {a : Eqv φ Γ (A, e)}
+  : (a.packed (Δ := Δ)).wk1 (inserted := inserted) = a.packed := wk_lift_packed (ρ := Ctx.InS.wk0)
+
+@[simp]
+theorem Eqv.wk2_packed {Γ Δ : Ctx α ε} {A : Ty α} {a : Eqv φ Γ (A, e)}
+  : (a.packed (Δ := V::Δ)).wk2 (inserted := inserted) = a.packed := by
+  simp only [wk2, <-Ctx.InS.lift_wk1, wk_lift_packed]
+
+@[simp]
+theorem Eqv.subst0_var0_packed {Γ Δ : Ctx α ε} {A : Ty α} {a : Eqv φ Γ (A, e)}
+  : a.packed.subst (var 0 Ctx.Var.shead).subst0 = a.packed (Δ := Δ)
+  := by rw [<-wk1_packed, subst0_var0_wk1]
+
 def Eqv.unpacked {Γ : Ctx α ε} (a : Eqv φ [(Γ.pack, ⊥)] (A, e)) (h : Γ.Pure)
   : Eqv φ Γ (A, e) := let1 (pack (by simp [h.effect])) (a.wk_id (by simp [Ctx.Wkn.drop]))
 
@@ -187,9 +233,9 @@ theorem Eqv.unpacked_def' {Γ : Ctx α ε} {a : Eqv φ [(Γ.pack, ⊥)] (A, e)} 
   simp [Subst.Eqv.get_comp]
 
 theorem Eqv.packed_wk0 {Γ : Ctx α ε} {a : Eqv φ Γ (A, e)}
-  : (a.wk0 (head := head)).packed (Δ := Δ) = pi_r ;;' a.packed := by
+  : (a.wk0 (head := head)).packed (Δ := Δ) = pi_l ;;' a.packed := by
   rw [
-    packed, wk0, <-subst_fromWk, subst_subst, seq, <-wk_eff_pi_r, let1_beta, wk1, <-subst_fromWk,
+    packed, wk0, <-subst_fromWk, subst_subst, seq, <-wk_eff_pi_l, let1_beta, wk1, <-subst_fromWk,
     subst_subst, packed, subst_subst
   ]
   congr 1; ext k
@@ -197,7 +243,7 @@ theorem Eqv.packed_wk0 {Γ : Ctx α ε} {a : Eqv φ Γ (A, e)}
     Set.mem_setOf_eq, Ctx.InS.coe_wk0, Nat.succ_eq_add_one, subst_var, id_eq,
     List.getElem_cons_succ, List.length_cons, Subst.Eqv.get_unpack, wk_res_self, ← subst_subst,
     subst_fromWk]
-  rw [<-wk1, wk1_pi_n, subst0_pi_r_pi_n]
+  rw [<-wk1, wk1_pi_n, subst0_pi_l_pi_n]
   rfl
 
 theorem Eqv.packed_packE {Γ : Ctx α ε} {h : Γ.Pure} : h.packE.packed (Δ := Δ) = nil (φ := φ) := by
@@ -206,8 +252,8 @@ theorem Eqv.packed_packE {Γ : Ctx α ε} {h : Γ.Pure} : h.packE.packed (Δ := 
   | cons V Γ I =>
     rw [packE_cons, packed_pair]
     convert Eqv.Pure.pair_eta _
-    · rfl
     · simp [packed_wk0, I]; rfl
+    · rfl
     · simp
 
 @[simp]
@@ -218,18 +264,18 @@ theorem Subst.Eqv.unpack_comp_packSE {Γ : Ctx α ε} (h : Γ.Pure)
     List.getElem_cons_zero, get_comp, get_packSE_zero, get_id, Fin.coe_fin_one]
   exact Eqv.packed_packE
 
-theorem Eqv.pi_n_eq_pi_n' {Γ Δ : Ctx α ε} (i : Fin Γ.length) :
-  Eqv.pi_n (φ := φ) (Δ := Δ) (e := e) i = Eqv.pi_n' i := by
-  induction Γ generalizing Δ with
-  | nil => exact i.elim0
-  | cons V Γ I =>
-  simp only [List.length_cons] at i
-  cases i using Fin.cases with
-  | zero => rfl
-  | succ =>
-    simp only [List.get_eq_getElem, List.length_cons, Fin.val_succ, List.getElem_cons_succ,
-      pi_n', Fin.val_zero, List.getElem_cons_zero, Fin.cases_succ, <-I]
-    rw [<-wk1_pi_n, <-wk1_pi_n, <-nil, <-pi_r_seq, pi_n_succ]
+-- theorem Eqv.pi_n_eq_pi_n' {Γ Δ : Ctx α ε} (i : Fin Γ.length) :
+--   Eqv.pi_n (φ := φ) (Δ := Δ) (e := e) i = Eqv.pi_n' i := by
+--   induction Γ generalizing Δ with
+--   | nil => exact i.elim0
+--   | cons V Γ I =>
+--   simp only [List.length_cons] at i
+--   cases i using Fin.cases with
+--   | zero => rfl
+--   | succ =>
+--     simp only [List.get_eq_getElem, List.length_cons, Fin.val_succ, List.getElem_cons_succ,
+--       pi_n', Fin.val_zero, List.getElem_cons_zero, Fin.cases_succ, <-I]
+--     rw [<-wk1_pi_n, <-wk1_pi_n, <-nil, <-pi_r_seq, pi_n_succ]
 
 theorem Eqv.unpacked_pi_n {Γ : Ctx α ε} {h : Γ.Pure} {i}
   : (Eqv.pi_n (φ := φ) (e := e) i).unpacked h = var i (h.any_effect_refl i.prop)
@@ -237,15 +283,18 @@ theorem Eqv.unpacked_pi_n {Γ : Ctx α ε} {h : Γ.Pure} {i}
   | nil => exact i.elim0
   | cons V Γ I => cases i using Fin.cases with
   | zero =>
-    simp [pi_n_zero, unpacked_def', pi_l, nil, subst_var, pl, Subst.Eqv.get_liftn₂_one]
-    rw [<-pl, pack, Pure.pl_pair]
+    simp [pi_n_zero, unpacked_def', pi_r, nil, subst_var, pr, Subst.Eqv.get_liftn₂_one]
+    rw [<-pr, pack, Pure.pr_pair]
     exact Pure.wk0 ⟨h.tail.packE, by simp⟩
   | succ i =>
     rw [unpacked_def', pi_n_succ, seq]
     simp only [List.get_eq_getElem, List.length_cons, Fin.val_succ, List.getElem_cons_succ,
       wk1_pi_n, subst_let1, subst_lift_pi_n]
-    simp [pi_r, pr, nil, subst_var]
-    rw [<-pr, pack, Pure.pr_pair, <-wk1_pi_n, <-wk0_let1, <-wk0_var]
+    simp only [pi_l, pl, nil, subst_let2, subst_var, List.getElem_cons_zero, List.length_singleton,
+      Fin.zero_eta, Fin.isValue, Subst.Eqv.get_packSE_zero, wk_res_eff, wk_eff_pack,
+      List.getElem_cons_succ, List.length_cons, Nat.reduceAdd, Fin.mk_one, Subst.Eqv.get_liftn₂_one,
+      List.get_eq_getElem, Fin.val_one, wk_eff_var]
+    rw [<-pl, pack, Pure.pl_pair, <-wk1_pi_n, <-wk0_let1, <-wk0_var]
     apply congrArg
     exact I (h := h.tail)
     exact ⟨var 0 (h.any_effect_refl (by simp)), rfl⟩
@@ -277,21 +326,20 @@ theorem Eqv.packed_var {Γ : Ctx α ε} {i} {hv}
 
 theorem Subst.Eqv.lift_unpack {Γ Δ : Ctx α ε}
   : (unpack (φ := φ) (Γ := Γ) (Δ := Δ)).lift (le_refl (A, ⊥))
-  = ((Eqv.var 0 (by simp)).pair (Eqv.var 1 (by simp))).subst0.comp Subst.Eqv.unpack := by
+  = ((Eqv.var 1 (by simp)).pair (Eqv.var 0 (by simp))).subst0.comp Subst.Eqv.unpack := by
   ext k
   cases k using Fin.cases with
   | zero =>
     simp [
-      Subst.Eqv.get_comp, Eqv.pi_n_zero, Eqv.pi_l, Eqv.nil, Eqv.pl, Eqv.let2_pair,
+      Subst.Eqv.get_comp, Eqv.pi_n_zero, Eqv.pi_r, Eqv.nil, Eqv.pr, Eqv.let2_pair,
       Eqv.let1_beta_var0, Eqv.let1_beta_var1]
   | succ k =>
     simp only [List.get_eq_getElem, List.length_cons, Fin.val_succ, List.getElem_cons_succ,
-      get_lift_succ, get_unpack, get_comp, Eqv.pi_n_succ, Eqv.seq, Eqv.pi_r, Eqv.pr, Eqv.nil,
+      get_lift_succ, get_unpack, get_comp, Eqv.pi_n_succ, Eqv.seq, Eqv.pi_l, Eqv.pl, Eqv.nil,
       Eqv.wk1_pi_n, Eqv.subst_let1, Eqv.subst_let2, Eqv.var0_subst0, Fin.zero_eta, Fin.val_zero,
-      List.getElem_cons_zero, Eqv.wk_res_eff, Eqv.wk_eff_pair, Eqv.wk_eff_var, ge_iff_le,
-      Prod.mk_le_mk, le_refl, bot_le, and_self, Eqv.subst_liftn₂_var_zero, Eqv.let2_pair,
-      Eqv.wk0_var, Nat.reduceAdd, Eqv.let1_beta_var0, Eqv.var_succ_subst0, Eqv.subst_lift_var_zero,
-      Eqv.let1_beta_var1, Nat.add_zero, Nat.zero_eq, Eqv.subst_lift_pi_n]
+      List.getElem_cons_zero, Eqv.wk_res_eff, Eqv.wk_eff_pair, Eqv.wk_eff_var,
+      Eqv.subst_liftn₂_var_one, Eqv.let2_pair, Eqv.wk0_var, zero_add, Eqv.let1_beta_var1,
+      Eqv.var_succ_subst0, Eqv.subst_lift_pi_n]
     rw [Eqv.wk0, <-Eqv.subst_fromWk]
     apply Eqv.eq_of_term_eq
     apply subst_eqOn_fvi
@@ -303,46 +351,46 @@ theorem Subst.Eqv.lift_unpack {Γ Δ : Ctx α ε}
 
 theorem Subst.Eqv.liftn₂_unpack {Γ Δ : Ctx α ε}
   : (unpack (φ := φ) (Γ := Γ) (Δ := Δ)).liftn₂ (le_refl (A, ⊥)) (le_refl (B, ⊥))
-  = (Eqv.pair (Eqv.var 0 (by simp))
-    (Eqv.pair (Eqv.var 1 (by simp)) (Eqv.var 2 (by simp)))).subst0.comp Subst.Eqv.unpack := by
+  = ((
+    Eqv.pair (Eqv.pair (Eqv.var 2 (by simp)) (Eqv.var 1 (by simp))) (Eqv.var 0 (by simp))
+  )).subst0.comp Subst.Eqv.unpack := by
   ext k
   cases k using Fin.cases with
   | zero =>
     simp only [List.get_eq_getElem, List.length_cons, Fin.val_zero, List.getElem_cons_zero,
-      get_liftn₂_zero, get_comp, get_unpack, Eqv.pi_n_zero, Eqv.pi_l, Eqv.pl, Eqv.nil,
-      Eqv.subst_let2, Eqv.var0_subst0, Fin.zero_eta, Eqv.wk_res_self, Eqv.subst_liftn₂_var_one,
-      Eqv.let2_pair, Eqv.wk0_pair, Eqv.wk0_var, Nat.reduceAdd, Eqv.let1_beta_var0, Eqv.subst_let1,
-      Eqv.subst_pair, Eqv.var_succ_subst0, Eqv.subst_lift_var_succ, zero_add]
+      get_liftn₂_zero, get_comp, get_unpack, Eqv.pi_n_zero, Eqv.pi_r, Eqv.pr, Eqv.nil,
+      Eqv.subst_let2, Eqv.var0_subst0, Fin.zero_eta, Eqv.wk_res_self, ge_iff_le, le_refl,
+      Eqv.subst_liftn₂_var_zero, Eqv.let2_pair, Eqv.wk0_var, zero_add, Eqv.let1_beta_var1]
     rw [Eqv.let1_beta'
-      (a' := (Eqv.pair (Eqv.var 1 (by simp)) (Eqv.var 2 (by simp)))) (h := by simp)]
+      (a' := (Eqv.pair (Eqv.var 2 (by simp)) (Eqv.var 1 (by simp)))) (h := by simp)]
     rfl
   | succ k =>
     cases k using Fin.cases with
     | zero =>
       simp [
-        Subst.Eqv.get_comp, Eqv.pi_n_zero, Eqv.pi_l, Eqv.nil, Eqv.pl, Eqv.let2_pair,
+        Subst.Eqv.get_comp, Eqv.pi_n_zero, Eqv.pi_r, Eqv.nil, Eqv.pl, Eqv.let2_pair,
         Eqv.let1_beta_var0, get_liftn₂_one,
       ]
-      rw [Eqv.pi_n_one, Eqv.seq_pi_l]
-      simp only [Eqv.pi_r, Eqv.subst_pl, Eqv.subst_pr, Eqv.nil_subst0, Eqv.wk_eff_self]
-      rw [Eqv.Pure.pr_pair, Eqv.Pure.pl_pair] <;> simp
+      rw [Eqv.pi_n_one, Eqv.seq_pi_r]
+      simp only [Eqv.pi_l, Eqv.subst_pl, Eqv.subst_pr, Eqv.nil_subst0, Eqv.wk_eff_self]
+      rw [Eqv.Pure.pl_pair, Eqv.Pure.pr_pair] <;> simp
     | succ k =>
       simp only [List.length_cons, List.get_eq_getElem, Fin.val_succ, List.getElem_cons_succ,
         get_liftn₂_succ, get_lift_succ, get_unpack, get_comp]
       rw [Eqv.pi_n_succ (Γ := _::Γ) (i := k.succ)]
       rw [Eqv.pi_n_succ]
       simp only [Eqv.seq, List.get_eq_getElem, List.length_cons, Fin.val_succ,
-        List.getElem_cons_succ, Eqv.pi_r, Eqv.nil, Eqv.wk1_pi_n, Eqv.wk1_let1, Eqv.wk1_pr,
+        List.getElem_cons_succ, Eqv.pi_l, Eqv.nil, Eqv.wk1_pi_n, Eqv.wk1_let1, Eqv.wk1_pl,
         Eqv.wk1_var0, Fin.zero_eta, Fin.val_zero, List.getElem_cons_zero, Eqv.wk2_pi_n,
-        Eqv.subst_let1, Eqv.subst_pr, Eqv.var0_subst0, Eqv.wk_res_eff, Eqv.wk_eff_pair,
+        Eqv.subst_let1, Eqv.subst_pl, Eqv.var0_subst0, Eqv.wk_res_eff, Eqv.wk_eff_pair,
         Eqv.wk_eff_var, Eqv.subst_lift_var_zero, Eqv.subst_lift_pi_n]
-      rw [Eqv.Pure.pr_pair]
+      rw [Eqv.Pure.pl_pair]
       rw [Eqv.let1_beta'
-        (a' := (Eqv.pair (Eqv.var 1 (by simp)) (Eqv.var 2 (by simp)))) (h := by simp)]
-      simp only [Eqv.subst_let1, Eqv.subst_pr, Eqv.var0_subst0, List.length_cons, Nat.add_zero,
+        (a' := (Eqv.pair (Eqv.var 2 (by simp)) (Eqv.var 1 (by simp)))) (h := by simp)]
+      simp only [Eqv.subst_let1, Eqv.subst_pl, Eqv.var0_subst0, List.length_cons, Nat.add_zero,
         Nat.zero_eq, Fin.zero_eta, List.get_eq_getElem, Fin.val_zero, List.getElem_cons_zero,
         Eqv.wk_res_eff, Eqv.wk_eff_pair, Eqv.wk_eff_var, Eqv.subst_lift_pi_n]
-      rw [Eqv.Pure.pr_pair, Eqv.let1_beta_var2, Eqv.wk0, Eqv.wk0, Eqv.wk_wk, <-Eqv.subst_fromWk]
+      rw [Eqv.Pure.pl_pair, Eqv.let1_beta_var2, Eqv.wk0, Eqv.wk0, Eqv.wk_wk, <-Eqv.subst_fromWk]
       apply Eqv.eq_of_term_eq
       apply subst_eqOn_fvi
       intro i
@@ -357,10 +405,10 @@ theorem Subst.Eqv.liftn₂_unpack {Γ Δ : Ctx α ε}
 theorem Eqv.packed_let1 {Γ : Ctx α ε} {A B : Ty α}
   {a : Eqv φ Γ (A, e)} {b : Eqv φ ((A, ⊥)::Γ) (B, e)}
   : (let1 a b).packed (Δ := Δ)
-  = let1 a.packed (let1 (pair (var 0 (by simp)) (var 1 (by simp))) b.packed) := by
+  = let1 a.packed (let1 (pair (var 1 (by simp)) (var 0 (by simp))) b.packed) := by
   rw [packed, subst_let1]; apply congrArg
   rw [
-    packed, let1_beta' (a' := pair (var 0 (by simp)) (var 1 (by simp))) (h := by simp),
+    packed, let1_beta' (a' := pair (var 1 (by simp)) (var 0 (by simp))) (h := by simp),
     subst_subst, Subst.Eqv.lift_unpack
   ]
 
@@ -368,12 +416,12 @@ theorem Eqv.packed_let2 {Γ : Ctx α ε} {A B C : Ty α}
   {a : Eqv φ Γ (A.prod B, e)} {b : Eqv φ ((B, ⊥)::(A, ⊥)::Γ) (C, e)}
   : (let2 a b).packed (Δ := Δ)
   = let2 a.packed (
-      let1 (pair (var 0 (by simp)) (pair (var 1 (by simp)) (var 2 (by simp)))) b.packed) := by
+      let1 (pair (pair (var 2 (by simp)) (var 1 (by simp))) (var 0 (by simp))) b.packed) := by
   rw [packed, subst_let2]; congr
   rw [
     packed,
     let1_beta'
-      (a' := (pair (var 0 (by simp)) (pair (var 1 (by simp)) (var 2 (by simp))))) (h := by simp),
+      (a' := pair (pair (var 2 (by simp)) (var 1 (by simp))) (var 0 (by simp))) (h := by simp),
     subst_subst, Subst.Eqv.liftn₂_unpack,
   ]
 
@@ -381,10 +429,10 @@ theorem Eqv.packed_case {Γ : Ctx α ε} {A B : Ty α}
   {a : Eqv φ Γ (A.coprod B, e)} {l : Eqv φ ((A, ⊥)::Γ) (C, e)} {r : Eqv φ ((B, ⊥)::Γ) (C, e)}
   : (case a l r).packed (Δ := Δ)
   = case a.packed
-    (let1 (pair (var 0 (by simp)) (var 1 (by simp))) l.packed)
-    (let1 (pair (var 0 (by simp)) (var 1 (by simp))) r.packed) := by
+    (let1 (pair (var 1 (by simp)) (var 0 (by simp))) l.packed)
+    (let1 (pair (var 1 (by simp)) (var 0 (by simp))) r.packed) := by
   rw [packed, subst_case]; congr <;> rw [
-    packed, let1_beta' (a' := pair (var 0 (by simp)) (var 1 (by simp))) (h := by simp),
+    packed, let1_beta' (a' := pair (var 1 (by simp)) (var 0 (by simp))) (h := by simp),
     subst_subst, Subst.Eqv.lift_unpack
   ]
 
