DeBruijnSSA/BinSyntax/Rewrite/Region/Compose/Structural/Product.lean
@@ -39,7 +39,7 @@ open Term.Eqv
 theorem Eqv.packed_in_let1 {Γ : Ctx α ε} {R : LCtx α}
   {a : Term.Eqv φ Γ (A, e)} {r : Eqv φ ((A, ⊥)::Γ) R}
   : (let1 a r).packed_in (Δ := Δ)
-  = let1 a.packed (let1 (pair (var 0 Ctx.Var.shead) (var 1 (by simp))) r.packed_in) := by
+  = let1 a.packed (let1 (pair (var 1 (by simp)) (var 0 Ctx.Var.shead)) r.packed_in) := by
   rw [packed_in, vsubst_let1]; apply congrArg
   rw [packed_in, let1_beta, vsubst_vsubst, Term.Subst.Eqv.lift_unpack]
 
@@ -47,7 +47,7 @@ theorem Eqv.packed_in_let2 {Γ : Ctx α ε} {R : LCtx α}
   {a : Term.Eqv φ Γ (A.prod B, e)} {r : Eqv φ ((B, ⊥)::(A, ⊥)::Γ) R}
   : (let2 a r).packed_in (Δ := Δ)
   = let2 a.packed (let1
-    (pair (var 0 Ctx.Var.shead) (pair (var 1 (by simp)) (var 2 (by simp))))
+    (pair (pair (var 2 (by simp)) (var 1 (by simp))) (var 0 Ctx.Var.shead))
     r.packed_in) := by
   rw [packed_in, vsubst_let2]; apply congrArg
   rw [packed_in, let1_beta, vsubst_vsubst, Term.Subst.Eqv.liftn₂_unpack]
@@ -56,15 +56,15 @@ theorem Eqv.packed_in_case {Γ : Ctx α ε} {R : LCtx α}
   {a : Term.Eqv φ Γ (A.coprod B, e)} {r : Eqv φ ((A, ⊥)::Γ) R} {s : Eqv φ ((B, ⊥)::Γ) R}
   : (case a r s).packed_in (Δ := Δ)
   = case a.packed
-    (let1 (pair (var 0 Ctx.Var.shead) (var 1 (by simp))) r.packed_in)
-    (let1 (pair (var 0 Ctx.Var.shead) (var 1 (by simp))) s.packed_in) := by
+    (let1 (pair (var 1 (by simp)) (var 0 Ctx.Var.shead)) r.packed_in)
+    (let1 (pair (var 1 (by simp)) (var 0 Ctx.Var.shead)) s.packed_in) := by
   rw [packed_in, vsubst_case]
   congr <;> rw [packed_in, let1_beta, vsubst_vsubst, Term.Subst.Eqv.lift_unpack]
 
 theorem Eqv.packed_in_cfg {Γ : Ctx α ε} {R L : LCtx α}
   {β : Eqv φ Γ (R ++ L)} {G}
   : (cfg R β G).packed_in (Δ := Δ)
-  = cfg R β.packed_in (λi => (let1 (pair (var 0 Ctx.Var.shead) (var 1 (by simp))) (G i).packed_in))
+  = cfg R β.packed_in (λi => (let1 (pair (var 1 (by simp)) (var 0 Ctx.Var.shead)) (G i).packed_in))
   := by
   rw [packed_in, vsubst_cfg]; apply congrArg; funext i
   rw [packed_in, let1_beta, vsubst_vsubst, Term.Subst.Eqv.lift_unpack]
