DeBruijnSSA/BinSyntax/Rewrite/Term/Compose/Completeness.lean
@@ -8,33 +8,100 @@ variable [Φ: EffInstSet φ (Ty α) ε] [PartialOrder α] [SemilatticeSup ε] [O
 
 namespace Term
 
--- theorem Eqv.packed_let1_den {Γ : Ctx α ε} {A B : Ty α}
---   {a : Eqv φ Γ (A, e)} {b : Eqv φ ((A, ⊥)::Γ) (B, e)}
---   : (let1 a b).packed (Δ := Δ)
---   = Eqv.split ;;' (a.packed ⋉' _) ;;' b.packed
---   := by
---   sorry
+theorem Eqv.packed_let1_den {Γ : Ctx α ε} {A B : Ty α}
+  {a : Eqv φ Γ (A, e)} {b : Eqv φ ((A, ⊥)::Γ) (B, e)}
+  : (let1 a b).packed (Δ := Δ) = Eqv.split ;;' (_ ⋊' a.packed) ;;' b.packed := by
+  rw [packed_let1, seq_rtimes, split, let2_pair, nil]
+  simp only [wk0_var, zero_add, wk1_packed, let1_beta_var0, subst_let1, var_succ_subst0, subst_pair,
+    subst_lift_var_succ, var0_subst0]
+  conv => rhs; rw [pair_bind, seq]
+  simp [let1_beta_var0, let1_let1]
 
--- theorem Eqv.packed_let2_den {Γ : Ctx α ε} {A B C : Ty α}
---   {a : Eqv φ Γ (A.prod B, e)} {b : Eqv φ ((B, ⊥)::(A, ⊥)::Γ) (C, e)}
---   : (let2 a b).packed (Δ := Δ)
---   = Eqv.split ;;' ((a.packed ;;' braid) ⋉' _) ;;' assoc ;;' b.packed := by
---   sorry
+theorem Eqv.packed_let2_den {Γ : Ctx α ε} {A B C : Ty α}
+  {a : Eqv φ Γ (A.prod B, e)} {b : Eqv φ ((B, ⊥)::(A, ⊥)::Γ) (C, e)}
+  : (let2 a b).packed (Δ := Δ) = Eqv.split ;;' (_ ⋊' a.packed) ;;' assoc_inv ;;' b.packed := by
+  rw [packed_let2, seq_rtimes, split, let2_pair, nil]
+  simp only [wk0_var, zero_add, let1_beta_var0, subst_let1, var_succ_subst0, subst_pair,
+    subst_lift_var_succ, var0_subst0, List.length_cons, Nat.reduceAdd, Fin.zero_eta,
+    List.get_eq_getElem, Fin.val_zero, List.getElem_cons_zero, wk_res_eff, wk_eff_var]
+  rw [seq_assoc_inv, reassoc_inv, let2_pair]
+  simp only [seq, let1_beta_var0, subst_let1, subst0_wk0, subst_let2, subst_lift_var_zero,
+    subst_pair, subst_liftn₂_var_add_2, subst_lift_var_succ, var0_subst0, List.length_cons,
+    Nat.reduceAdd, Fin.zero_eta, List.get_eq_getElem, Fin.val_zero, List.getElem_cons_zero,
+    wk_res_eff, wk_eff_var, wk0_var, zero_add, subst_liftn₂_var_one, ge_iff_le, Prod.mk_le_mk,
+    le_refl, bot_le, and_self, subst_liftn₂_var_zero, let1_let1, let1_let2]
+  rw [let2_bind]
+  simp only [wk2, wk_let1, wk_pair, wk_var, Set.mem_setOf_eq, Ctx.InS.coe_wk2, Nat.liftnWk,
+    lt_self_iff_false, ↓reduceIte, le_refl, tsub_eq_zero_of_le, Nat.succ_eq_add_one, zero_add,
+    Nat.reduceAdd, Nat.one_lt_ofNat, zero_lt_two, wk1_packed, subst_lift_packed, subst0_var0_packed]
+  congr
+  exact wk_lift_packed
 
--- theorem Eqv.packed_case_den {Γ : Ctx α ε} {A B : Ty α}
---   {a : Eqv φ Γ (A.coprod B, e)} {l : Eqv φ ((A, ⊥)::Γ) (C, e)} {r : Eqv φ ((B, ⊥)::Γ) (C, e)}
---   : (case a l r).packed (Δ := Δ)
---   = Eqv.split ;;' (a.packed ⋉' _) ;;' distr_inv ;;' sorry := by
---   sorry
+theorem Eqv.packed_case_den {Γ : Ctx α ε} {A B : Ty α}
+  {a : Eqv φ Γ (A.coprod B, e)} {l : Eqv φ ((A, ⊥)::Γ) (C, e)} {r : Eqv φ ((B, ⊥)::Γ) (C, e)}
+  : (case a l r).packed (Δ := Δ)
+  = Eqv.split ;;' (_ ⋊' a.packed) ;;' distl_inv ;;' coprod l.packed r.packed := by
+  rw [packed_case, seq_rtimes, split, let2_pair, nil]
+  simp only [wk0_var, zero_add, wk1_packed, let1_beta_var0, subst_let1, var_succ_subst0, subst_pair,
+    subst_lift_var_succ, var0_subst0, List.length_cons, Nat.reduceAdd, Fin.zero_eta,
+    List.get_eq_getElem, Fin.val_zero, List.getElem_cons_zero, wk_res_eff, wk_eff_var,
+    subst_lift_packed, subst0_var0_packed]
+  conv => rhs; rw [distl_inv, seq, seq, let1_pair]
+  simp only [let1_beta_let2_eta, nil, coprod, wk1_inl, wk1_pair, wk1_var_succ, zero_add, wk1_var0,
+    List.length_cons, Fin.zero_eta, List.get_eq_getElem, Fin.val_zero, List.getElem_cons_zero,
+    wk1_inr, wk1_let2, wk_case, wk_var, Set.mem_setOf_eq, Ctx.InS.coe_liftn₂, Nat.liftnWk,
+    zero_lt_two, ↓reduceIte, wk_inl, wk_pair, Ctx.InS.coe_lift, Ctx.InS.coe_wk1, Nat.liftWk_succ,
+    Nat.one_lt_ofNat, Nat.reduceAdd, Nat.liftWk_zero, wk_inr, subst_let2, var0_subst0, wk_res_eff,
+    wk_eff_pair, wk_eff_var, subst_case, ge_iff_le, Prod.mk_le_mk, le_refl, bot_le, and_self,
+    subst_liftn₂_var_zero, subst_inl, subst_pair, subst_lift_var_succ, subst_liftn₂_var_one,
+    wk0_var, subst_lift_var_zero, subst_inr, let2_pair, let1_beta_var1, var_succ_subst0,
+    ↓dreduceIte, Nat.succ_eq_add_one, Nat.reduceSub, let1_beta_var0, subst_let1, subst0_wk0,
+    wk1_packed, wk1_case, wk2_packed, let1_let1, let1_case]
+  rw [case_bind]
+  congr
+  · rw [let1_beta' (a' := (pair (var 2 (by simp)) (var 0 (by simp))).inl) (h := by simp)]
+    simp only [subst_case, var0_subst0, List.length_cons, Fin.zero_eta, List.get_eq_getElem,
+      Fin.val_zero, List.getElem_cons_zero, wk_res_eff, wk_eff_inl, wk_eff_pair, wk_eff_var,
+      case_inl]
+    rw [let1_beta' (a' := (pair (var 2 (by simp)) (var 0 (by simp)))) (h := by simp)]
+    induction l using Quotient.inductionOn
+    apply eq_of_term_eq
+    simp only [Set.mem_setOf_eq, InS.coe_wk, Ctx.InS.coe_wk1, InS.coe_subst, InS.coe_subst0,
+      InS.coe_pair, InS.coe_var, Subst.InS.coe_unpack, Term.subst_subst, ← Term.subst_fromWk,
+      Subst.InS.coe_lift, InS.coe_inl]
+    congr
+    funext k; simp only [Subst.comp, Term.subst_lift_pi_n, Subst.pi_n, Term.subst_subst]
+    apply subst_eqOn_fvi
+    intro x
+    rw [fvi_pi_n]
+    simp only [Set.mem_Iio, Nat.lt_one_iff]
+    intro h; cases h; rfl
+  · rw [let1_beta' (a' := (pair (var 2 (by simp)) (var 0 (by simp))).inr) (h := by simp)]
+    simp only [subst_case, var0_subst0, List.length_cons, Fin.zero_eta, List.get_eq_getElem,
+      Fin.val_zero, List.getElem_cons_zero, wk_res_eff, wk_eff_inr, wk_eff_pair, wk_eff_var,
+      case_inr]
+    rw [let1_beta' (a' := (pair (var 2 (by simp)) (var 0 (by simp)))) (h := by simp)]
+    induction r using Quotient.inductionOn
+    apply eq_of_term_eq
+    simp only [Set.mem_setOf_eq, InS.coe_wk, Ctx.InS.coe_wk1, InS.coe_subst, InS.coe_subst0,
+      InS.coe_pair, InS.coe_var, Subst.InS.coe_unpack, Term.subst_subst, ← Term.subst_fromWk,
+      Subst.InS.coe_lift, InS.coe_inl]
+    congr
+    funext k; simp only [Subst.comp, Term.subst_lift_pi_n, Subst.pi_n, Term.subst_subst]
+    apply subst_eqOn_fvi
+    intro x
+    rw [fvi_pi_n]
+    simp only [Set.mem_Iio, Nat.lt_one_iff]
+    intro h; cases h; rfl
 
--- @[simp]
--- theorem Eqv.packed_inl_den {Γ : Ctx α ε} {A B : Ty α} {a : Eqv φ Γ (A, e)}
---   : (inl (B := B) a).packed (Δ := Δ) = inl a.packed := sorry
+@[simp]
+theorem Eqv.packed_inl_den {Γ : Ctx α ε} {A B : Ty α} {a : Eqv φ Γ (A, e)}
+  : (inl (B := B) a).packed (Δ := Δ) = a.packed ;;' inj_l := by rw [seq_inj_l, packed_inl]
 
--- @[simp]
--- theorem Eqv.packed_inr_den {Γ : Ctx α ε} {A B : Ty α} {a : Eqv φ Γ (B, e)}
---   : (inr (A := A) a).packed (Δ := Δ) = inr a.packed := sorry
+@[simp]
+theorem Eqv.packed_inr_den {Γ : Ctx α ε} {A B : Ty α} {a : Eqv φ Γ (B, e)}
+  : (inr (A := A) a).packed (Δ := Δ) = a.packed ;;' inj_r := by rw [seq_inj_r, packed_inr]
 
--- @[simp]
--- theorem Eqv.packed_abort_den {Γ : Ctx α ε} {A : Ty α} {a : Eqv φ Γ (Ty.empty, e)}
---   : (abort a A).packed (Δ := Δ) = abort a.packed A := sorry
+@[simp]
+theorem Eqv.packed_abort_den {Γ : Ctx α ε} {A : Ty α} {a : Eqv φ Γ (Ty.empty, e)}
+  : (abort a A).packed (Δ := Δ) = a.packed ;;' zero := by rw [seq_zero, packed_abort]
